-new UpToC-notion for time bounds -finished rduction from multi to mono-tape

theories/L/Complexity/Reductions/TMGenNP/mTM_to_singleTapeTM.v
@@ -6,7 +6,7 @@ From Undecidability.TM Require TM ProgrammingTools CaseList.
 
 
 From Undecidability.L.Complexity  Require GenNP.
-From Undecidability.L.Complexity  Require Import LMGenNP TMGenNP_fixed_mTM.
+From Undecidability.L.Complexity  Require Import LMGenNP TMGenNP_fixed_mTM M_multi2mono.
 
 
 From Undecidability.TM.Single Require EncodeTapes StepTM DecodeTapes. (** In emacs: coq-prefer-top-of-conclusion: t; *)
@@ -15,458 +15,64 @@ Unset Printing Coercions.
 From Coq.ssr Require ssrfun.
 Module Option := ssrfun.Option.
 
-Module MultiToMono.
-  Section multiToMono.
-
-    (** We can simulate any machine while first testing that we indeed work on a valid n-tape encoding *)
-
-    Import EncodeTapes DecodeTapes Single.StepTM ProgrammingTools Combinators Decode.
-    Context (sig F:finType) (n:nat) (M__multi : pTM sig F n).
-
-    Definition M : pTM ((sigList (sigTape sig)) ^+) (option F) 1 :=
-      If (CheckTapeContains.M (CheckEncodesTapes.M n))
-         (Move L;;If (Relabel ReadChar (Option.apply (fun _ => false) true))
-                     (Move R;;Relabel (ToSingleTape M__multi) Some)
-                     (Return Nop None))
-         (Return Nop None).
-
-    Definition Rel : pRel ((sigList (sigTape sig)) ^+) (option F) 1 :=
-      fun t '(y,t') => match y with
-                      None => ~ exists (v : tapes sig n), StepTM.contains_tapes t[@Fin0] v
-                    | Some y => exists (v v': tapes sig n), StepTM.contains_tapes t[@Fin0] v
-                                                      /\ StepTM.contains_tapes t'[@Fin0] v'
-                                                      /\ Canonical_Rel M__multi v (y,v')
-                    end.
-
-    Lemma Realises : M ⊨ Rel .
-    Proof.
-      intros H__multi.
-      eapply Realise_monotone.
-      {unfold M. TM_Correct.
-       -apply CheckTapeContains.Realises. now apply CheckEncodesTapes.Realises. exact _.
-       -eapply ToSingleTape_Realise', Canonical_Realise.
-      }  
-      intros t (y,t'). cbn in *.
-      intros [H|H];unfold Rel;cbn.
-      2:{ destruct H as (?&([Henc]&_)&->&_&<-). intros (v&Hv). hnf in Hv. inversion Henc. apply H.
-          exists v,[]. rewrite Hv. now rewrite Encode_map_id. } 
-      destruct H as (?&[[Henc] <-]&_&t1&Ht1&H). 2:easy.
-      destruct H as [H|H].
-      2:{ destruct H as (?&(?&?&->&<-)&->&_&<-). rewrite Ht1 in H. intros (v&Ht). hnf in Ht.
-          rewrite Ht in H. now cbn in H. }
-      destruct H as (?&(?&Hc1&->&->)&(_&t2&Ht2&y'&->&Hm)).
-      rewrite Ht1 in Ht2. destruct (current t1[@Fin0]) eqn:Hc1';inv Hc1.
-      inv Henc. rename H into Henc. destruct Henc as (x'&t__L&Henc). rewrite Encode_map_id in Henc.
-      erewrite tape_move_left_right in Ht2. 2:now rewrite Henc.
-      rewrite Ht2 in *. clear Ht2 t2. rewrite Ht1 in *. clear Ht1 t1.
-      destruct t__L. 2:now rewrite Henc in Hc1'.
-      specialize Hm with (1:=Henc) as (?&(?&?&?&<-&<-)&?).
-      do 3 eexists. exact Henc. split. eauto.
-      unfold Canonical_T;eauto. 
-    Qed.
-
-    Context (T__multi : tRel sig n).
-
-    Definition Ter : tRel ((sigList (sigTape sig)) ^+) 1 :=
-      fun t k  => exists (k' k__sim: nat), (forall (v : tapes sig n),
-                                   StepTM.contains_tapes t[@Fin0] v
-                                   -> T__multi v k__sim
-                                     /\ Loop_steps (start (projT1 M__multi)) v k__sim <= k')
-                               /\ ((| right t[@Fin0] |)*4*(n+1) + n*16 + 27 + k') <= k .
-
-    Lemma Terminates  : projT1 M__multi ↓ T__multi -> projT1 M ↓ Ter.
-    Proof.
-      intros H__multi.
-      eapply TerminatesIn_monotone.
-      {unfold M. TM_Correct.
-       -apply CheckTapeContains.Realises. now apply CheckEncodesTapes.Realises. exact _.
-       -eapply CheckTapeContains.Terminates. now apply CheckEncodesTapes.Realises. apply CheckEncodesTapes.Terminates.
-       -eapply ToSingleTape_Terminates'. eassumption.
-      }  
-      intros t k (k'&k__sim&Hk__sim&Hk). infTer 2. infTer 2. hnf. reflexivity.
-      split. shelve.
-      intros ? b [Henc Hbeq]. destruct b. 2:now apply Nat.le_0_l.
-      infTer 4. intros t1 [] Ht1. cbn in Ht1.
-      infTer 4. cbn. intros t2 b (?&Hb&->&->).
-      destruct b. 2:now apply Nat.le_0_l.
-      infTer 4. intros t2 _ Ht2. hnf.
-      destruct Henc. inv H. rename H0 into Henc. destruct Henc as (v&t__L&Heq).
-      rewrite Ht1 in Ht2. specialize (Hbeq eq_refl). subst tout. cbn in *.
-      rewrite Heq in Ht1. rewrite Ht1 in Hb. destruct t__L;inv Hb. rewrite Heq in Ht2. cbn in Ht2.
-      rewrite Ht2. clear Ht2 Ht1 t1 t2.
-      edestruct Hk__sim as (H__k&Hk__sim').  1:{ hnf. rewrite Heq. now rewrite map_id. }
-      eexists v,_. split. 1:{ hnf. now rewrite map_id. }
-      split. eassumption. eassumption.
-      Unshelve. cbn - [plus mult]. rewrite CheckEncodesTapes.length_right_tape_move_right. cbn - [plus mult].
-      ring_simplify.
-      transitivity ((| right t[@Fin0] |)*4*(n+1) + n*16 + 27 + k'). cbn - [plus mult].
-      nia. exact Hk. 
-    Qed.
-(*
-    Definition Ter' : tRel ((sigList (sigTape sig)) ^+) 1 :=
-      fun t k  => exists (k' k__sim: nat), (forall (v : tapes sig n),
-                                   StepTM.contains_tapes t[@Fin0] v
-                                   -> Canonical_T (projT1 M__multi) v k__sim
-                                     /\ Loop_steps (start (projT1 M__multi)) v k__sim <= k')
-                               /\ ((| right t[@Fin0] |)*4*(n+1) + n*16 + 27 + k') <= k .
-
-    Local Arguments Canonical_T : simpl never. 
-    Lemma Terminates'  : projT1 M ↓ Ter'.
-    Proof.
-      intros H__multi.
-      eapply TerminatesIn_monotone.
-      {unfold M. TM_Correct.
-       -apply CheckTapeContains.Realises. now apply CheckEncodesTapes.Realises. exact _.
-       -eapply CheckTapeContains.Terminates. now apply CheckEncodesTapes.Realises. apply CheckEncodesTapes.Terminates.
-       -eapply ToSingleTape_Terminates'. eapply Canonical_TerminatesIn.
-      }  
-      intros t k (k'&k__sim&Hk__sim&Hk). infTer 2. infTer 2. hnf. reflexivity.
-      split. shelve.
-      intros ? b [Henc Hbeq]. destruct b. 2:now apply Nat.le_0_l.
-      infTer 4. intros t1 [] Ht1. cbn in Ht1.
-      infTer 4. cbn. intros t2 b (?&Hb&->&->).
-      destruct b. 2:now apply Nat.le_0_l.
-      infTer 4. intros t2 _ Ht2. hnf.
-      destruct Henc. inv H. rename H0 into Henc. destruct Henc as (v&t__L&Heq).
-      rewrite Ht1 in Ht2. specialize (Hbeq eq_refl). subst tout. cbn in *.
-      rewrite Heq in Ht1. rewrite Ht1 in Hb. destruct t__L;inv Hb. rewrite Heq in Ht2. cbn in Ht2.
-      rewrite Ht2. clear Ht2 Ht1 t1 t2.
-      edestruct Hk__sim as (H__k&Hk__sim').  1:{ hnf. rewrite Heq. now rewrite map_id. }
-      eexists v,_. split. 1:{ hnf. now rewrite map_id. }
-      split. eassumption. eassumption.
-      Unshelve. cbn - [plus mult]. rewrite CheckEncodesTapes.length_right_tape_move_right. cbn - [plus mult].
-      ring_simplify.
-      transitivity ((| right t[@Fin0] |)*4*(n+1) + n*16 + 27 + k'). cbn - [plus mult].
-      nia. exact Hk. 
-    Qed. 
-    *)
-  End multiToMono.
-End MultiToMono.
-Arguments MultiToMono.Rel : simpl never.
-Arguments MultiToMono.Ter : simpl never.
-
-
-(*****************************************************************)
-(* Module Diverge.                                               *)
-(*   Section Diverge.                                            *)
-(*                                                               *)
-(*     Import ProgrammingTools While.                            *)
-(*     Context {sig:finType} {n:nat}.                              *)
-(*     Definition M : pTM sig unit n := While (Return Nop None). *)
-(*                                                               *)
-(*     Lemma Realises : M ⊨ (fun _ _ => False).                         *)
-(*     Proof.                                                    *)
-(*       eapply Realise_monotone. 1:{unfold M. TM_Correct. }     *)
-(*       apply WhileInduction. all:cbn. all:easy.                *)
-(*     Qed.                                                      *)
-(*   End Diverge.                                                *)
-(* End Diverge.                                                  *)
-(*****************************************************************)
-
+From Undecidability Require Import TapeFuns.
 Import LTactics GenEncode CodeTM EncodeTapes.
-  
-Run TemplateProgram (tmGenEncode "boundary_enc" boundary).
-Hint Resolve boundary_enc_correct : Lrewrite.
-
-Section sigList.
-  Context (sig : Type) `{H:registered sig}.
-  Run TemplateProgram (tmGenEncode "sigList_enc" (sigList sig)).
-
-  Global Instance term_sigList_X : computableTime' (@sigList_X sig) (fun _ _ => (1,tt)).
-  Proof. extract constructor. solverec.
-  Qed.
-
-End sigList.
-Hint Resolve sigList_enc_correct : Lrewrite.
-
-
-Section sigTape.
-  Context (sig : Type) `{H:registered sig}.
-  Run TemplateProgram (tmGenEncode "sigTape_enc" (sigTape sig)).
-End sigTape.
-Hint Resolve sigTape_enc_correct : Lrewrite.
-
 
 From Undecidability Require Import Datatypes.Lists.
 
+Import EncodeTapes DecodeTapes Single.StepTM ProgrammingTools Combinators Decode.
+Import LTactics LSum LProd LVector LNat Lists.
+
+Import EqBool.
+
+
+From Undecidability Require Import MultiUnivTimeSpaceSimulation.
+
+From Undecidability Require Import UpToCNary LTactics.
+
+Lemma mapTime_upTo X (t__f : X -> nat):
+  map_time t__f <=c (fun l => length l + sumn (map t__f l) + 1 ).
+Proof.
+  unfold map_time. exists 12.
+  induction x;cbn - [plus mult]. all: nia.
+Qed.
+
+Lemma size_finType_any_le (X:finType) `{registered X} (x:X):
+  L.size (enc x) <= maxl (map (fun x => L.size (enc x)) (elem X)).
+Proof.
+  apply maxl_leq. eauto.
+Qed.
+
+Lemma size_finType_any_le_c (X:finType) `{registered X}:
+  (fun x => L.size (enc x)) <=c (fun _ => 1).
+Proof.
+  setoid_rewrite size_finType_any_le. smpl_upToC_solve.
+Qed.
+
+Lemma  ptc_sizeOfmtapes sig n `{registered sig}:
+  polyTimeComputable (@sizeOfmTapes sig n).
+Proof.
+  
+Admitted.
+
+
+Import M_multi2mono.
+
+
 Section LMGenNP_to_TMGenNP_mTM.
-  Import EncodeTapes DecodeTapes Single.StepTM ProgrammingTools Combinators Decode.
-  Import LTactics LSum LProd LVector LNat Lists.
+
 
   Context (sig:finType) (n:nat) `{R__sig : registered sig}  (M : mTM sig (S n)).
 
-  
-  Definition putFirstAtEnd n: Vector.t (Fin.t (S n)) (S n):=
-    tabulate (fun i => match lt_dec (S (proj1_sig (Fin.to_nat i))) (S n) with
-                      Specif.left H => Fin.of_nat_lt H
-                    | _ => Fin.F1
-                    end).
-  Arguments putFirstAtEnd : simpl never.
-
-  Definition putEndAtFirst n': Vector.t (Fin.t (S n')) (S n'). 
-    refine (tabulate (fun i => match Fin.to_nat i with
-                    | exist _ 0 H => Fin.of_nat_lt (Nat.lt_succ_diag_r n')
-                    | exist _ n' H => Fin.of_nat_lt (p:=n'-1) _
-                            end )). abstract nia.
-  Defined.
-  Arguments putEndAtFirst : simpl never.
-
-  Section printFin.
-    Local Arguments Fin.t : clear implicits.
-    Local Arguments Fin.FS : clear implicits.
-    Local Arguments Fin.F1 : clear implicits.
-    Local Arguments Vector.cast : clear implicits.
-
-    Lemma putFirstAtEnd_dupfree m: dupfree (putFirstAtEnd m).
-    Proof.
-      clear_all. apply dupfree_tabulate_injective.
-      intros i j. destruct (Fin.to_nat i) as [i' Hi] eqn:eqi. destruct (Fin.to_nat j) as [j' Hj] eqn:eqj .
-      cbn. 1:do 2 destruct lt_dec. 2,3:easy.
-      2:{ intros _. apply Fin.to_nat_inj. rewrite eqi. rewrite eqj. cbn. clear eqi eqj. nia. }
-      intros H%Fin.FS_inj. apply Fin.to_nat_inj.
-      rewrite eqi,eqj. cbn. specialize (lt_S_n _ _ l) as H1. specialize (lt_S_n _ _ l0) as H2.
-      erewrite <- (Fin.of_nat_ext H1), <- (Fin.of_nat_ext H2) in H.
-      apply(f_equal Fin.to_nat) in H. rewrite !Fin.to_nat_of_nat in H.
-      now inv H.
-    Qed.
-    
-    Lemma putEndAtFirst_dupfree m: dupfree (putEndAtFirst m).
-    Proof.
-      clear_all. apply dupfree_tabulate_injective.
-      intros i j.
-      destruct (Fin.to_nat i) eqn:?;destruct (Fin.to_nat j) eqn:?; cbn in *.
-      eassert (H'1:=Heqs). assert (H'2:=Heqs0).
-      erewrite <- (Fin.of_nat_to_nat_inv i) in Heqs. erewrite <- (Fin.of_nat_to_nat_inv j) in Heqs0. 
-      rewrite Fin.to_nat_of_nat in Heqs. rewrite Fin.to_nat_of_nat in Heqs0. inversion Heqs; inversion Heqs0.
-            destruct (fin_destruct_S i) as [ (i'&->) | ->]; destruct (fin_destruct_S j) as [ (j'&->) | ->].
-            all:try change (Fin.FS m i') with (Fin.R 1 i') in *; try change (Fin.FS m j') with (Fin.R 1 j') in *.
-            all:change (S m) with (1+m) in *.
-            all: rewrite ?Fin.R_sanity in H0;rewrite ?Fin.R_sanity in H1. all: subst;cbn.
-            all:intros Heq%(f_equal Fin.to_nat).
-            all:rewrite !Fin.to_nat_of_nat in Heq. 
-            all:inversion Heq as [H2]. all:try rewrite ?Nat.sub_0_r in H2.
-            all:try apply Fin.to_nat_inj in H2. all:try easy.
-      -clear - l H2.  nia.
-      -clear - l0 H2.  nia.
-    Qed.
-    
-  End printFin.
-  
-  Definition M__mono : pTM ((sigList (sigTape sig)) ^+) unit 1 :=
-    If (Move R ;; Relabel (MultiToMono.M (LiftTapes (M;(fun _ => tt)) (putEndAtFirst n) )) (Option.apply (fun _ => true) false))
-       Nop
-       Diverge.
-
   Local Arguments Canonical_Rel : simpl never. 
-  Lemma Realises__mono:
-    M__mono ⊨(fun tin '(_,tout) =>
-              exists v v' : tapes sig (S n),
-                contains_tapes (tape_move_right tin[@Fin0]) v /\
-                contains_tapes tout[@Fin0] v' /\
-                Canonical_Rel (LiftTapes (existT (fun x : mTM sig (S n) => states x -> unit) M (fun _ : states M => tt)) (putEndAtFirst n)) v
-                              (tt, v')).
-  Proof.
-    eapply Realise_monotone.
-    { unfold M__mono. TM_Correct. apply MultiToMono.Realises. } cbn.
-    intros tin ([],tout). cbn. intros [H|H].
-    2:now decompose record H.
-    destruct H as (?&([]&t1&Ht1&b&Hb&H__mono)&<-). destruct b as [ [] | ] ;inv Hb.
-    hnf in H__mono. cbn - [Canonical_Rel]in *|-*. rewrite Ht1 in *|-*. easy.
-  Qed.
-  
-    Lemma Terminates_False sig' n' (M' : mTM sig' n'): M' ↓ (fun _ _ => False).
-  Proof.
-    easy.
-  Qed.
-  
-
-  Lemma Terminates__mono:
-    projT1 M__mono ↓ (fun t k => exists (v : tapes _ (S n)) k',
-                        contains_tapes (tape_move_right t[@Fin0]) v
-                        /\ MultiToMono.Ter (LiftTapes (existT _ M (fun _  => tt)) (putEndAtFirst n))
-                                          (LiftTapes_T (putEndAtFirst n) (Canonical_T M))
-                                          [|(tape_move_right t[@Fin0])|] k'
-                        /\ k' + 3 <= k).
-  Proof.
-    eapply TerminatesIn_monotone.
-    { unfold M__mono. TM_Correct.
-      -apply MultiToMono.Realises.
-      -eapply MultiToMono.Terminates. apply LiftTapes_Terminates. apply putEndAtFirst_dupfree. eapply Canonical_TerminatesIn.
-      -apply Terminates_False.
-    }
-    intros tin k (v&k'&Hv&HT&Hk). cbn.
-    infTer 7. intros t1 _ Ht1. unfold tapes in *. destruct_vector;cbn in *. subst h. apply HT. shelve.
-    intros tout b (?&t1&Ht1&[[]| ]&->&Hr). all:cbn. 2:{ apply Hr. cbn in *. rewrite <- Ht1 in *. easy. } reflexivity.
-    Unshelve.
-    { rewrite <- Hk. nia. } (*
-    hnf in Hr. destruct Hr as (v0&v'&Hv0&Hv'&Hr). replace v0 with v in * by admit.
-    hnf in Hr. cbnunfold LiftTapes in Hr.  cbn in Hr.
-    (*TODO: move trivial relation in Realisation so we get that M terminated if M__Mono halted. *)
-    destruct r
-    2:now decompose record H.
-    destruct H as (?&(b&Hf&H)&<-).
-    destruct b as [[]| ];inv Hf. 
-    destruct H as (v&v'&Hv&Hv'&HR&_).
-    do 3 eexists. 2:split. all:eassumption. *)
-  Qed.
   
   
 
-  (*MOVE*)
-  Lemma sizeOfTape_encodeTape sig' (t : tape sig') :
-  | encode_tape t | = let l := sizeOfTape t in if 0 =? l then 1 else 2 + sizeOfTape t.
-  Proof.
-    destruct t;cbn - [Nat.eqb].
-    all:repeat (autorewrite with list;cbn [length]).
-    1:easy.
-    2,3:rewrite !Nat.add_succ_r. all:cbn [Nat.eqb]. all:nia.
-  Qed.
-
+  Let M__mono := M__mono M.
   
-  Lemma sizeOfTape_encodeTape_le sig' (t : tape sig') :
-  | encode_tape t | <= 2 + sizeOfTape t.
-  Proof.
-    rewrite sizeOfTape_encodeTape. cbn;destruct _;nia.
-  Qed.
+  Arguments MultiToMono.Rel : simpl never.
+  Arguments MultiToMono.Ter : simpl never.
 
-  Import EqBool.
-
-  Lemma encode_list_concat sigX X (cX : codable sigX X) l:
-    encode_list cX l = concat (map (fun t => sigList_cons :: map sigList_X (encode t)) l) ++[sigList_nil].
-  Proof.
-    induction l;cbn. reflexivity.
-    rewrite IHl. cbn. now autorewrite with list.
-  Qed.
-
-  Lemma list_eq_nth_error X (xs ys : list X) :
-    (forall n, nth_error xs n = nth_error ys n) -> xs = ys.
-  Proof.
-    induction xs in ys|-*;destruct ys;cbn;intros H. 1:easy. 1-2:now specialize (H 0).
-    generalize (H 0).  intros [= ->]. erewrite IHxs. easy. intros n'. now specialize (H (S n')).
-  Qed.
-
-  Lemma vector_nth_error X n' i (xs : Vector.t X n') :
-    nth_error (Vector.to_list xs) i = match lt_dec i n' with
-                                        Specif.left H => Some (Vector.nth xs (Fin.of_nat_lt H))
-                                      | _ => None
-                                      end.
-  Proof.
-    clear. rewrite <- vector_to_list_correct. induction xs in i|-*. now destruct i.
-    cbn in *. destruct i;cbn. easy. rewrite IHxs. do 2 destruct lt_dec. 4:easy. now symmetry;erewrite Fin.of_nat_ext. all:exfalso;nia. 
-  Qed.
-    
-
-  Lemma putFirstAtEnd_to_list X n' (x:X) xs:
-    (Vector.to_list (select (putFirstAtEnd n') (x ::: xs))) = Vector.to_list xs ++ [x].
-  Proof.
-    clear. apply list_eq_nth_error. intros i.
-    rewrite !vector_nth_error. destruct lt_dec.
-    { rewrite select_nth. unfold putFirstAtEnd. rewrite nth_tabulate,Fin.to_nat_of_nat;cbn.
-      destruct lt_dec.
-      -erewrite nth_error_app1. 2:now rewrite TMunflatten.vector_to_list_length.
-       cbn. rewrite vector_nth_error. destruct lt_dec. 2:exfalso;nia.
-       erewrite Fin.of_nat_ext. reflexivity.
-      -cbn. rewrite nth_error_app2. all:rewrite TMunflatten.vector_to_list_length. 2:nia. replace (i-n') with 0 by nia. easy.
-    }
-    symmetry. apply nth_error_None. erewrite app_length, TMunflatten.vector_to_list_length. cbn;nia.
-  Qed.
-
-  Lemma putEnd_invL X (v : Vector.t X _) :
-    select (putEndAtFirst n) (select (putFirstAtEnd n) v) = v.
-  Proof.
-    apply Vector.eq_nth_iff. intros i ? <-. rewrite !select_nth.
-    f_equal. 
-    unfold putEndAtFirst,putFirstAtEnd. rewrite !nth_tabulate.
-    destruct (fin_destruct_S i) as  [(i'&->) | ->].
-    2:{ cbn. rewrite Fin.to_nat_of_nat. cbn. destruct lt_dec. now exfalso;nia. easy. }
-    eapply Fin.to_nat_inj.
-    remember (Fin.to_nat (Fin.FS i')) as i0 eqn:H. set (tmp:=proj1_sig i0).
-    rewrite (sig_eta i0). subst tmp i0. cbn.
-    destruct (Fin.to_nat i') eqn:H.
-    cbn. rewrite Fin.to_nat_of_nat;cbn. destruct lt_dec;cbn.
-    -rewrite (sig_eta (Fin.to_nat _)). cbn. rewrite Fin.to_nat_of_nat. cbn. nia.
-    -clear H. nia.
-  Qed.
-
-  
-  Lemma right_sizeOfTape sig' (t:tape sig') :
-    length (right t) <= sizeOfTape t.
-  Proof.
-    destruct t;cbn. all:autorewrite with list;cbn. all:nia.
-  Qed.
-  
-
-
-  From Undecidability Require Import MultiUnivTimeSpaceSimulation.
-  Lemma size_list X sigX (cX: codable sigX X) (l:list X) :
-    size l = sumn (map size l) + length l + 1.
-  Proof.
-    unfold size. cbn. rewrite encode_list_concat.
-    rewrite app_length, length_concat, map_map. cbn.
-    change S with (fun x => 1 + x). rewrite sumn_map_add,sumn_map_c. setoid_rewrite map_length.
-    cbn.  nia.
-  Qed.
-
-  Lemma concat_eq_inv_borderL X isBorder xs R__L ys b (R__R : list X):
-    (forall x, x el xs -> exists hd tl, x = hd::tl /\ isBorder hd /\ forall c, c el tl -> ~isBorder c) ->
-    (forall x, x el ys -> exists hd tl, x = hd::tl /\ isBorder hd /\ forall c, c el tl -> ~isBorder c) ->
-    (forall x, x el R__R -> ~isBorder x) ->
-    isBorder b ->
-    concat xs ++ b::R__L = concat ys++R__R ->
-    (forall i, i < length xs -> nth_error xs i = nth_error ys i) /\ b::R__L = concat (skipn (length xs) ys) ++ R__R.
-  Proof.
-    clear. induction xs as [ | x xs] in ys|-*;intros HL HR HRR Hb Heq.
-    { cbn in *. easy. }
-    destruct ys as [ |y ys].
-    { exfalso. cbn in Heq. subst R__R.
-      destruct (HL x) as (?&?&->&?&?). easy. eapply HRR. 2:easy. cbn;easy. }
-    cbn in Heq. autorewrite with list in Heq.
-    destruct (HL x) as (x__hd&x__tl&->&Hxhd&Hxtl). easy.
-    destruct (HR y) as (y__hd&y__tl&->&_&Hytl). easy.
-    cbn in *. 
-    revert Heq. intros [= <- Heq].
-    replace y__tl with x__tl in *.
-    2:{ induction x__tl as [ | x' xtl] in y__tl,Heq,HL,HR,Hytl,Hxtl|-*.
-        -destruct y__tl. easy. cbn in Heq. destruct xs.
-         +now edestruct (Hytl x);inv Heq.
-         +edestruct (HL l) as (?&?&->&?&?). easy. inv Heq. now edestruct Hytl.
-        -destruct y__tl.
-         2:{ inv Heq. f_equal. eapply IHxtl. 3-5:cbn;intros;auto.
-             all:intros z [<-| ].  all:now eauto 7. 
-         }
-         exfalso. destruct ys. 2:{ edestruct (HR l) as (?&?&->&?&?). easy. inv Heq. cbn in *. now eapply Hxtl. }
-         cbn in Heq. 
-         inv Heq. eapply HRR. 2:exact Hb. eauto 10.
-    }
-    apply app_inv_head in Heq. apply IHxs in Heq.  2-5:now eauto 7.
-    destruct Heq as (IH&->). split. 2:easy.
-    intros [] ?. easy. cbn. apply IH. nia.
-  Qed.
-
-  Lemma vector_app_to_list X k k' (xs : Vector.t X k) (ys : Vector.t X k'):
-    vector_to_list (Vector.append xs ys) = vector_to_list xs ++ vector_to_list ys.
-  Proof.   
-    induction xs. easy. cbn. congruence.
-  Qed.
-
-  Lemma putEndAtFirst_to_list X n' v (ts:X) v0:
-    Vector.to_list v ++ [ts] = Vector.to_list v0 ->
-    select (putEndAtFirst n') v0 = ts ::: v.
-  Admitted.
-
-  Instance term_concat X `{registered X}: computableTime' (@concat X) (fun l _ => (cnst ("todo",l),tt)).
-  Admitted.
-
-  
-  Instance term_encode_tape X `{registered X}: computableTime' (@encode_tape X) (fun l _ => (cnst ("todo: encode_tape",l),tt)).
-  Admitted.
-
-  Lemma contains_tapes_inj (sig' : finType) n' t (v v' : tapes sig' n'):
-    contains_tapes t v -> contains_tapes t v' -> v = v'.
-  Proof.
-    unfold contains_tapes. intros -> [= eq]. apply app_inv_tail in eq. apply map_injective in eq. 2:congruence.
-    eassert (H':=encode_prefixInjective (t:=[]) (t':=[])). rewrite !app_nil_r in H'. apply H' in eq. easy.
-  Qed.
   
   Local Arguments loopM : clear implicits.
   Local Arguments loopM {_ _ } _ _ _. 
@@ -474,28 +80,33 @@ Section LMGenNP_to_TMGenNP_mTM.
     restrictBy (HaltsOrDiverges_fixed_mTM M) (TMGenNP_fixed_mTM M)
                ⪯p unrestrictedP (TMGenNP_fixed_singleTapeTM (projT1 M__mono)).
   Proof.
-    evar (f__steps : nat -> nat -> nat -> nat). unfold TMGenNP_fixed_mTM. unfold TMGenNP_fixed_singleTapeTM. cbn.
+    subst M__mono.
+    evar (f__steps : nat*nat*nat -> nat). evar (f__nice : nat*nat*nat -> nat).
+    enough (Hf__nice : f__steps <=c f__nice).
+    unfold TMGenNP_fixed_mTM. unfold TMGenNP_fixed_singleTapeTM. cbn.
     set (t__start:=fun (ts : tapes sig n) => inl START::concat (map (fun t => inr (sigList_cons)::map (fun s => inr (sigList_X s)) (encode_tape t)) (Vector.to_list ts))++[inr (sigList_cons)]).
+    set (t__size := fun maxSize => 3 + if eqb 0 maxSize then 0 else 1 + maxSize).
     eapply reducesPolyMO_intro_restrictBy with
         (f:=fun '(ts,maxSize,steps) => (t__start ts
-                                     ,3 + if eqb 0 maxSize then 0 else 1 + maxSize
-                                     ,f__steps steps (sizeOfmTapes ts) maxSize+ 3)).
-    2:{ intros [[v maxSize] steps]. unfold HaltsOrDiverges_fixed_mTM. intros H_HaltOrDiv.
+                                     ,t__size maxSize
+                                     ,  c__leUpToC (H:=Hf__nice) * f__nice (steps,sizeOfmTapes ts,maxSize)+ 3)).
+    2:{ unfold execTM.
+        intros [[v maxSize] steps]. unfold HaltsOrDiverges_fixed_mTM. intros H_HaltOrDiv.
         split. easy. split.
-        -intros (t1&Ht1&s__end&Hs__end). cbn.
-         eexists _,(map (fun c => inr (sigList_X c)) (encode_tape t1) ++ [inr sigList_nil;inl STOP]). split. now subst t__start. 
-         split. 1:{ autorewrite with list. rewrite sizeOfTape_encodeTape. cbn - [Nat.eqb].
+        -intros (t1&Ht1&s__end&Hs__end).
+         eexists (map (fun c => inr (sigList_X c)) (encode_tape t1) ++ [inr sigList_nil;inl STOP]). 
+         split. 1:{ cbn - [plus]. autorewrite with list. rewrite sizeOfTape_encodeTape. cbn - [Nat.eqb].
                     destruct (Nat.eqb_spec 0 (sizeOfTape t1));
                       destruct (eqb_spec 0 (maxSize)). all:try nia.
          }
          edestruct Terminates__mono as (?&?).
-         2:{ eexists. rewrite H. easy. }
+         2:{ eexists. cbn. unfold execTM. rewrite H. easy. }
          cbn. set (tin:=midtape _ _ _).
          eexists (select (putFirstAtEnd n) (t1:::v)), _.
          assert (Ht1v:contains_tapes tin (select (putFirstAtEnd n) (t1 ::: v))). 
          { hnf. subst tin. f_equal. unfold encode_tapes.
            rewrite encode_list_concat.
-           autorewrite with list. cbn.  rewrite !concat_map,!map_map.
+           autorewrite with list. cbn. rewrite !concat_map,!map_map.
            rewrite vector_to_list_correct,putFirstAtEnd_to_list.
            autorewrite with list. cbn. repeat setoid_rewrite map_map.
            rewrite concat_app;cbn. autorewrite with list. easy.
@@ -506,23 +117,28 @@ Section LMGenNP_to_TMGenNP_mTM.
           split. 1: {hnf. rewrite putEnd_invL. eauto. }
           assert (H':=proj2_sig M2MBounds.Loop_steps_nice). hnf in H'.
           unfold PrettyBounds.dominatedWith in H'.
-          rewrite H'. cbn in *. rewrite vector_to_list_correct, putFirstAtEnd_to_list.
+          rewrite H'. rewrite vector_to_list_correct, putFirstAtEnd_to_list.
           rewrite BaseCode.encodeList_size_app,size_list, to_list_length.
-          unfold size. cbn - [mult plus].
+          unfold size. cbn - [mult plus]. 
           autorewrite with list. cbn [length]. rewrite sizeOfTape_encodeTape_le.
           erewrite sumn_map_le_pointwise with (f2:=fun x => _).
           2:{ intros. rewrite sizeOfTape_encodeTape_le. rewrite sizeOfmTapes_upperBound. 2:now eapply tolist_In. reflexivity. }
           rewrite !sumn_map_c,to_list_length.
-          reflexivity.
-         +cbn - [mult plus]. autorewrite with list;cbn - [plus mult].
+          unshelve erewrite ( _ : (n * (2 + sizeOfmTapes v) + n + 1 + S (2 + sizeOfTape t1 + 1) + S n * steps)
+                                  <= ((steps + sizeOfmTapes v + 5)* S n + sizeOfTape t1)). nia.
+          reflexivity. 
+         +cbn - [mult plus]. autorewrite with list; cbn - [plus mult].
           rewrite length_concat,map_map;cbn - [plus mult];setoid_rewrite map_length.
           rewrite sizeOfTape_encodeTape_le,Ht1.
           rewrite sumn_le_bound.
           2:{ intros ? (?&<-&?)%in_map_iff.
               rewrite sizeOfTape_encodeTape_le, sizeOfmTapes_upperBound. 2:now apply tolist_In. reflexivity. }
-          rewrite map_length. rewrite to_list_length. [f__steps]:intros ? ? ?.
+          rewrite map_length. rewrite to_list_length.
+          replace (1 + (2 + maxSize + 2)) with (maxSize + 5) by lia.
+          setoid_rewrite <- correct__leUpToC.
+          [f__steps]:refine (fun '(steps, sizeOfmTapes, maxSize) =>  _).
           set (sizeOfmTapes _). unfold f__steps. reflexivity.
-        -intros (c__hs&t1&Hhd&Hsize&f&Hf). cbn - [mult plus] in *. inv Hhd. 
+        -intros (cert&Hsize&f'&Hf'). destruct @loopM as [f| ] eqn:Hf. all:cbn -[plus mult t__start] in *. 2:now inv Hf'. clear Hf' f'.
          apply Realises__mono in Hf as (v0&v1&Hv0&Hv1&H__mono). cbn in Hv0.
          hnf in H__mono;cbn in H__mono. unfold LiftTapes in H__mono;cbn in H__mono.
          destruct H__mono as (outc&k&Hout&<-&_).
@@ -536,7 +152,7 @@ Section LMGenNP_to_TMGenNP_mTM.
          2,3:now split;[easy | intros ? (y&<-&Hiny)%in_map_iff;easy].
          destruct H' as [Hinit Hlast]. rewrite <- utils.map_skipn in Hlast.
          destruct (split_vector v0 n) as (v'&vlst) eqn:Hsplit.
-         unshelve eassert (H':=split_vector_correct _ _). 6:rewrite Hsplit in H'. abstract nia.
+         unshelve eassert (H':=split_vector_correct _ _). 6:rewrite Hsplit in H'. clear. abstract nia. 
          cbn [fst snd] in H'.  apply (f_equal (@vector_to_list _ _ )) in H'. rewrite vector_to_list_cast in H'. clear Hsplit.
          rewrite vector_app_to_list in H'.  
          revert v' vlst H'. replace (Init.Nat.min n (S n)) with n by nia. replace (S n - n) with 1 by nia.
@@ -560,25 +176,174 @@ Section LMGenNP_to_TMGenNP_mTM.
          rewrite skipn_app in Hlast. 2:now rewrite to_list_length. cbn in Hlast.
          autorewrite with list in Hlast. cbn in Hlast. revert Hlast. intros [= ->].
          exists ts. assert (Hts__size : sizeOfTape ts <= maxSize).
-         1:{ autorewrite with list in Hsize.  rewrite sizeOfTape_encodeTape in Hsize.
+         1:{ autorewrite with list in Hsize.  rewrite sizeOfTape_encodeTape in Hsize. unfold t__size in *.
              destruct (eqb_spec 0 maxSize);destruct sizeOfTape. all:cbn in Hsize;try nia. }
          clear Hsize. split. easy. unfold initc in *. cbn in Hout.
          unshelve eassert (Htmp := LiftTapes_lift _ _). 11:{ now rewrite Hout. } now apply putEndAtFirst_dupfree.
          cbn in Htmp. unfold selectConf in Htmp. cbn in Htmp.
 
-         erewrite putEndAtFirst_to_list in Htmp. 2:exact eq.
+         erewrite putEndAtFirst_to_list in Htmp. 2:exact eq. 
          eexists. setoid_rewrite loop_monotone. 2:eassumption. reflexivity. 
          eapply H_HaltOrDiv. all:eassumption.
     }
-    evar (time : nat -> nat). [time]:intros n0.
-    eexists.
-    { unfold f__steps, t__start. 
-      From Undecidability Require Import L.TM.TMflatComp.
-      Fail Intern.extractAs t. 
-      admit.
-
+    2:{
+      
+      unfold f__steps.
+      enough ((fun _ => 1) <=c f__nice).
+      smpl_upToC.
+      3:{ [f__nice]: exact (fun '(x,y,z) => (fun s => s*s*S x) (S x + y + z)).
+          subst f__nice.
+          set (c:= 5*(S n) + 1).
+          exists (c * c).
+          intros [[x y] z].
+          set (s:=S x+y+z).  
+          unshelve erewrite (_ : (x + y + 5) * S n + z <= c*s). 1:{ unfold s,c. nia. }
+          nia.
+      }
+      all:unfold f__nice. all:smpl_upToC_solve.
     }
 
-  Admitted.
+    assert (polyTimeComputable f__nice).
+    { 
+      evar (time : nat -> nat). [time]:intros n0.
+      eexists (fun x => time x).
+      { unfold f__nice. extract. solverec.
+        set (n0:=(L.size (enc (a0, b0, b)))).
+        assert (a0+b0+b+1 <= n0). 1:{ unfold n0. rewrite !size_prod. cbn [fst snd]. rewrite !size_nat_enc. nia. }
+        unshelve erewrite (_ : a0 <= n0). nia. unshelve erewrite (_ : b0 <= n0). nia. unshelve erewrite (_ : b <= n0). nia.
+        unfold time. reflexivity. }
+      1,2:unfold time;smpl_inO.
+      { evar (f__size : nat -> nat). [f__size]:intros n0. exists f__size.
+        { intros [[a0 b0] b]. unfold f__nice.
+          set (n0:=(L.size (enc (a0, b0, b)))).
+          assert (a0+b0+b+1 <= n0). 1:{ unfold n0. rewrite !size_prod. cbn [fst snd]. rewrite !size_nat_enc. nia. }
+          rewrite size_nat_enc. 
+          unshelve erewrite (_ : a0 <= n0). nia. unshelve erewrite (_ : b0 <= n0). nia. unshelve erewrite (_ : b <= n0). nia.
+          change S with (plus 1).
+          unfold f__size;reflexivity.
+        }
+        all:unfold f__size;smpl_inO.
+      }
+    }
+    clearbody f__nice.
+
+    assert (polyTimeComputable t__size).
+    { 
+      evar (c0 : nat).
+      eexists (fun _ => c0).
+      { unfold t__size. extract. solverec. all:rewrite eqbTime_le_l.
+        all:set (c:=L.size (enc 0)). all:cbv in c;subst c. all:subst c0. 2:easy. nia. }
+      1,2:smpl_inO.
+      { evar (f__size : nat -> nat). [f__size]:intros n0. exists f__size.
+        { intros x. unfold t__size.
+          set (n0:=(L.size (enc x))).
+          assert (Hx:x<=n0) by apply size_nat_enc_r.
+          rewrite size_nat_enc. destruct _. 2:rewrite Hx;unfold f__size;reflexivity. unfold f__size. nia.
+        }
+        
+        all:unfold f__size;smpl_inO.
+      }
+    }clearbody t__size.
+
+    assert (polyTimeComputable t__start).
+    {
+      set (f:=fun s : sigTape sig => inr (sigList_X s)) in t__start.
+      assert ( {f__c:UpToC (fun _ => 1) & computableTime' f (fun _ _ => (f__c tt,tt))}) as [t__f comp__f].
+      {  evar (c:nat). exists_UpToC (fun _ => c). unfold f. clear_all. extract. solverec. [c]:exact 3. now unfold c. subst c. smpl_upToC_solve. }
+
+      set (g:= (fun t : tape sig => inr sigList_cons :: map f (encode_tape t))) in t__start.
+      assert ( {t__g:UpToC (fun t=> sizeOfTape t + 1) & computableTime' g (fun t _ => (t__g t,tt))}) as [t__g comp__g].
+      {  evar (t__c: tape sig -> nat). [t__c]:intro. exists_UpToC t__c. unfold g.
+         extract. solverec.
+         rewrite map_time_const,sizeOfTape_encodeTape_le. all:unfold t__c. reflexivity. smpl_upToC_solve.
+      } 
+      
+      evar (time : nat -> nat). [time]:intros n0.
+      eexists (fun x => time x).
+      { unfold t__start. extract. solverec. rewrite (UpToC_le _).
+        rewrite (correct__leUpToC (mapTime_upTo _)). 
+        rewrite length_concat,map_map. subst g. cbn -[plus mult]. setoid_rewrite map_length. rewrite to_list_length.
+        erewrite sumn_map_le_pointwise  with (f2:=fun _ => _).
+        2:{ intros;rewrite (UpToC_le t__g),sizeOfmTapes_upperBound;try reflexivity;now apply tolist_In. }
+        erewrite sumn_map_le_pointwise with (f1:=fun x1 : tape sig => S (| encode_tape x1 |)) (f2:=fun _ => _).
+        2:{ intros. setoid_rewrite sizeOfTape_encodeTape_le at 1. rewrite sizeOfmTapes_upperBound at 1. 2:now apply tolist_In.
+            reflexivity. }
+        rewrite sumn_map_c,to_list_length.
+        rewrite sumn_map_c,to_list_length.
+        rewrite TMEncoding.sizeOfmTapes_by_size. set (L.size _).
+        unfold time. reflexivity.
+      }
+      1,2:now unfold time;change S with (plus 1);smpl_inO.
+      { evar (f__size : nat -> nat). [f__size]:intros n0. exists f__size.
+        { intros x. unfold t__start.
+          rewrite size_list_cons. subst g f.
+          rewrite Lists.size_list. rewrite map_app,concat_map,map_map. cbn. setoid_rewrite map_map. rewrite sumn_app.
+          assert (H' : forall l, sumn (concat l) = sumn (map sumn l)). 1:{induction l;cbn;now autorewrite with list. }
+          rewrite H',map_map. cbn. set (tmp:=L.size (enc (inr sigList_cons)));cbv in tmp;subst tmp.
+          setoid_rewrite size_sum. rewrite size_boundary. setoid_rewrite size_sigList.
+          repeat setoid_rewrite <- plus_assoc.  ring_simplify. ring_simplify (7 + (4 + 5)).
+          repeat setoid_rewrite sumn_map_add. repeat setoid_rewrite sumn_map_c. setoid_rewrite sumn_map_mult_c_r.
+          setoid_rewrite sumn_map_le_pointwise with (f2:=fun x => _)at 2.
+          2:{ setoid_rewrite sizeOfTape_encodeTape_le at 1;intros;rewrite sizeOfmTapes_upperBound at 1. 2:now apply tolist_In. reflexivity. }
+          rewrite sumn_map_c.
+          setoid_rewrite sumn_map_le_pointwise with (f2:=fun x => _).
+          2:{ intros. setoid_rewrite sumn_map_le_pointwise with (f2:=fun x => _).
+              2:{ intros. apply (correct__leUpToC (size_finType_any_le_c (X:=finType_CS (sigTape sig)))). }
+              rewrite sumn_map_c. rewrite sizeOfTape_encodeTape_le,  sizeOfmTapes_upperBound. 2:now apply tolist_In. reflexivity. }
+          rewrite sumn_map_c. rewrite to_list_length. setoid_rewrite TMEncoding.sizeOfmTapes_by_size.
+          set (n0:= L.size _). ring_simplify. unfold f__size. reflexivity.
+        }
+        all:unfold f__size;smpl_inO.
+      }
+    }
+    clearbody f__steps t__start.
+(*    assert (polyTimeComputable (@sizeOfmTapes sig n)) by apply ptc_sizeOfmtapes. *)
+
+    evar (time : nat -> nat). [time]:intros n0.
+      eexists (fun x => time x).
+      {
+        extract. solverec.
+        remember (L.size (enc (a0, b0, b))) as n0 eqn:Hn0.
+        rewrite !size_prod in Hn0. cbn [fst snd] in Hn0.
+        erewrite (mono__polyTC _ (x':=n0)). 2:{ subst n0. repeat set (L.size _). nia. }
+        setoid_rewrite (mono__polyTC _ (x':=n0)) at 2. 2:{ subst n0. repeat set (L.size _). nia. } 
+        assert (H'' : L.size (enc (b, sizeOfmTapes a0, b0)) <= n0*5).
+        {  rewrite !size_prod. cbn [fst snd]. setoid_rewrite size_nat_enc at 2.
+            rewrite TMEncoding.sizeOfmTapes_by_size. subst n0. repeat set (L.size _). nia. }
+        setoid_rewrite (mono__polyTC _ (x':=n0*5)) at 3. 2:exact H''. 
+        specialize (bounds__rSP (f:=f__nice)) as H'. setoid_rewrite <- size_nat_enc_r in H'.
+        unshelve rewrite H'. now apply resSize__polyTC.
+        setoid_rewrite mono__rSP. 2:exact H''.
+        rewrite TMEncoding.sizeOfmTapes_by_size at 1. unshelve erewrite (_ : L.size (enc a0) <= n0). now (subst n0;clear;repeat set (L.size _);nia).
+        unfold time. reflexivity.
+      }
+      1,2:now unfold time;smpl_inO;apply inOPoly_comp;smpl_inO.
+      { evar (f__size : nat -> nat). [f__size]:intros n0. exists f__size.
+        { intros [[a0 b0] b]. remember (L.size (enc (a0, b0, b))) as n0 eqn:Hn0.
+          rewrite !size_prod in Hn0|-*. cbn [fst snd] in Hn0|-*. rewrite !size_nat_enc.
+          assert (H'' : L.size (enc (b, sizeOfmTapes a0, b0)) <= n0*5).
+        {  rewrite !size_prod. cbn [fst snd]. setoid_rewrite size_nat_enc at 2.
+           rewrite TMEncoding.sizeOfmTapes_by_size. subst n0. repeat set (L.size _). nia. }
+        specialize (bounds__rSP (f:=f__nice)) as H'. setoid_rewrite <- size_nat_enc_r in H'.
+        unshelve rewrite H'. now apply resSize__polyTC.
+        setoid_rewrite mono__rSP. 2:exact H''.
+
+        specialize (bounds__rSP (f:=t__size)) as Hsize. setoid_rewrite <- size_nat_enc_r in Hsize at 1.
+        unshelve rewrite Hsize. now apply resSize__polyTC. 
+        setoid_rewrite (mono__rSP _ (x':=n0)) at 1 . 2:nia.
+
+        specialize (bounds__rSP (f:=t__start)) as Hstart.
+        unshelve rewrite Hstart. now apply resSize__polyTC. 
+        setoid_rewrite (mono__rSP _ (x':=n0)) at 1 . 2:subst;clear;repeat (set (L.size _));nia.
+        unfold f__size. reflexivity.
+        }
+        1,2:unfold f__size;smpl_inO; apply inOPoly_comp;smpl_inO.
+
+      }
+    
+        
+  Qed.
+
+  Print Assumptions LMGenNP_to_TMGenNP_mTM. 
 
 End LMGenNP_to_TMGenNP_mTM.
