theories/L/Complexity/Reductions/TMGenNP/M_multi2mono.v
@@ -1,0 +1,549 @@
+From Undecidability.L Require Import Tactics.LTactics.
+From Undecidability.L.Datatypes Require Import Lists LVector.
+From Undecidability.L.Complexity Require Import NP Synthetic Monotonic.
+From Undecidability.TM Require Import TM.
+From Undecidability.TM Require TM ProgrammingTools CaseList.
+
+
+From Undecidability.L.Complexity  Require GenNP.
+From Undecidability.L.Complexity  Require Import LMGenNP TMGenNP_fixed_mTM.
+
+
+From Undecidability.TM.Single Require EncodeTapes StepTM DecodeTapes. (** In emacs: coq-prefer-top-of-conclusion: t; *)
+
+Unset Printing Coercions.
+From Coq.ssr Require ssrfun.
+Module Option := ssrfun.Option.
+
+Module MultiToMono.
+  Section multiToMono.
+
+    (** We can simulate any machine while first testing that we indeed work on a valid n-tape encoding *)
+
+    Import EncodeTapes DecodeTapes Single.StepTM ProgrammingTools Combinators Decode.
+    Context (sig F:finType) (n:nat) (M__multi : pTM sig F n).
+
+    Definition M : pTM ((sigList (sigTape sig)) ^+) (option F) 1 :=
+      If (CheckTapeContains.M (CheckEncodesTapes.M n))
+         (Move L;;If (Relabel ReadChar (Option.apply (fun _ => false) true))
+                     (Move R;;Relabel (ToSingleTape M__multi) Some)
+                     (Return Nop None))
+         (Return Nop None).
+
+    Definition Rel : pRel ((sigList (sigTape sig)) ^+) (option F) 1 :=
+      fun t '(y,t') => match y with
+                      None => ~ exists (v : tapes sig n), StepTM.contains_tapes t[@Fin0] v
+                    | Some y => exists (v v': tapes sig n), StepTM.contains_tapes t[@Fin0] v
+                                                      /\ StepTM.contains_tapes t'[@Fin0] v'
+                                                      /\ Canonical_Rel M__multi v (y,v')
+                    end.
+
+    Lemma Realises : M ⊨ Rel .
+    Proof.
+      intros H__multi.
+      eapply Realise_monotone.
+      {unfold M. TM_Correct.
+       -apply CheckTapeContains.Realises. now apply CheckEncodesTapes.Realises. exact _.
+       -eapply ToSingleTape_Realise', Canonical_Realise.
+      }  
+      intros t (y,t'). cbn in *.
+      intros [H|H];unfold Rel;cbn.
+      2:{ destruct H as (?&([Henc]&_)&->&_&<-). intros (v&Hv). hnf in Hv. inversion Henc. apply H.
+          exists v,[]. rewrite Hv. now rewrite Encode_map_id. } 
+      destruct H as (?&[[Henc] <-]&_&t1&Ht1&H). 2:easy.
+      destruct H as [H|H].
+      2:{ destruct H as (?&(?&?&->&<-)&->&_&<-). rewrite Ht1 in H. intros (v&Ht). hnf in Ht.
+          rewrite Ht in H. now cbn in H. }
+      destruct H as (?&(?&Hc1&->&->)&(_&t2&Ht2&y'&->&Hm)).
+      rewrite Ht1 in Ht2. destruct (current t1[@Fin0]) eqn:Hc1';inv Hc1.
+      inv Henc. rename H into Henc. destruct Henc as (x'&t__L&Henc). rewrite Encode_map_id in Henc.
+      erewrite tape_move_left_right in Ht2. 2:now rewrite Henc.
+      rewrite Ht2 in *. clear Ht2 t2. rewrite Ht1 in *. clear Ht1 t1.
+      destruct t__L. 2:now rewrite Henc in Hc1'.
+      specialize Hm with (1:=Henc) as (?&(?&?&?&<-&<-)&?).
+      do 3 eexists. exact Henc. split. eauto.
+      unfold Canonical_T;eauto. 
+    Qed.
+
+    Context (T__multi : tRel sig n).
+
+    Definition Ter : tRel ((sigList (sigTape sig)) ^+) 1 :=
+      fun t k  => exists (k' k__sim: nat), (forall (v : tapes sig n),
+                                   StepTM.contains_tapes t[@Fin0] v
+                                   -> T__multi v k__sim
+                                     /\ Loop_steps (start (projT1 M__multi)) v k__sim <= k')
+                               /\ ((| right t[@Fin0] |)*4*(n+1) + n*16 + 27 + k') <= k .
+    Lemma Terminates  : projT1 M__multi ↓ T__multi -> projT1 M ↓ Ter.
+    Proof.
+      intros H__multi.
+      eapply TerminatesIn_monotone.
+      {unfold M. TM_Correct.
+       -apply CheckTapeContains.Realises. now apply CheckEncodesTapes.Realises. exact _.
+       -eapply CheckTapeContains.Terminates. now apply CheckEncodesTapes.Realises. apply CheckEncodesTapes.Terminates.
+       -eapply ToSingleTape_Terminates'. eassumption.
+      }  
+      intros t k (k'&k__sim&Hk__sim&Hk). infTer 2. infTer 2. hnf. reflexivity.
+      split. shelve.
+      intros ? b [Henc Hbeq]. destruct b. 2:now apply Nat.le_0_l.
+      infTer 4. intros t1 [] Ht1. cbn in Ht1.
+      infTer 4. cbn. intros t2 b (?&Hb&->&->).
+      destruct b. 2:now apply Nat.le_0_l.
+      infTer 4. intros t2 _ Ht2. hnf.
+      destruct Henc. inv H. rename H0 into Henc. destruct Henc as (v&t__L&Heq).
+      rewrite Ht1 in Ht2. specialize (Hbeq eq_refl). subst tout. cbn in *.
+      rewrite Heq in Ht1. rewrite Ht1 in Hb. destruct t__L;inv Hb. rewrite Heq in Ht2. cbn in Ht2.
+      rewrite Ht2. clear Ht2 Ht1 t1 t2.
+      edestruct Hk__sim as (H__k&Hk__sim').  1:{ hnf. rewrite Heq. now rewrite map_id. }
+      eexists v,_. split. 1:{ hnf. now rewrite map_id. }
+      split. eassumption. eassumption.
+      Unshelve. cbn - [plus mult]. rewrite CheckEncodesTapes.length_right_tape_move_right. cbn - [plus mult].
+      ring_simplify.
+      transitivity ((| right t[@Fin0] |)*4*(n+1) + n*16 + 27 + k'). cbn - [plus mult].
+      abstract nia. exact Hk. 
+    Qed.
+  End multiToMono.
+End MultiToMono.
+Arguments MultiToMono.Rel : simpl never.
+Arguments MultiToMono.Ter : simpl never.
+
+Import LTactics GenEncode CodeTM EncodeTapes.
+  
+Run TemplateProgram (tmGenEncode "boundary_enc" boundary).
+Hint Resolve boundary_enc_correct : Lrewrite.
+
+Lemma size_boundary (l:boundary):
+  L.size (enc l) = match l with START => 6 | STOP => 5 | UNKNOWN => 4 end.
+Proof.
+  change (enc l) with (boundary_enc l). 
+  destruct l;easy.
+Qed.
+
+Section sigList.
+  Context (sig : Type) `{H:registered sig}.
+  Run TemplateProgram (tmGenEncode "sigList_enc" (sigList sig)).
+
+  Global Instance term_sigList_X : computableTime' (@sigList_X sig) (fun _ _ => (1,tt)).
+  Proof. extract constructor. solverec.
+  Qed.
+
+  
+
+  Lemma size_sigList (l:sigList sig):
+    L.size (enc l) = match l with sigList_X x => L.size (enc x) + 7 | sigList_nil => 5 | _ => 4 end.
+  Proof.
+    change (enc l) with (sigList_enc l).
+    destruct l. all:cbn [sigList_enc map sumn size].
+    change ((match _ with
+             | @mk_registered _ enc _ _ => enc
+             end s)) with (enc s).
+    all:cbn;nia. 
+  Qed.
+
+
+End sigList.
+Hint Resolve sigList_enc_correct : Lrewrite.
+
+
+Section sigTape.
+  Context (sig : Type) `{H:registered sig}.
+  Run TemplateProgram (tmGenEncode "sigTape_enc" (sigTape sig)).
+
+  Global Instance term_LeftBlank_X : computableTime' (@LeftBlank sig) (fun _ _ => (1,tt)).
+  Proof. extract constructor. solverec. Qed.
+
+  Global Instance term_RightBlank_X : computableTime' (@RightBlank sig) (fun _ _ => (1,tt)).
+  Proof. extract constructor. solverec. Qed.
+
+  Global Instance term_MarkedSymbol_X : computableTime' (@MarkedSymbol sig) (fun _ _ => (1,tt)).
+  Proof. extract constructor. solverec. Qed.
+
+  Global Instance term_UnmarkedSymbol_X : computableTime' (@UnmarkedSymbol sig) (fun _ _ => (1,tt)).
+  Proof. extract constructor. solverec. Qed.
+
+  
+  Lemma size_sigTape (l:sigTape sig):
+    L.size (enc l) =
+    match l with
+      LeftBlank b => 11+ L.size (enc b)
+    | RightBlank b => 10+ L.size (enc b)
+    | NilBlank => 8
+    | MarkedSymbol x => 8 + L.size (enc x)
+    | UnmarkedSymbol x => 7 + L.size (enc x)
+    end.
+  Proof.
+    change (enc l) with (sigTape_enc l).
+    destruct l. all:cbn [sigTape_enc map sumn size].
+    1-2:unfold enc;cbn.
+    4-5:change ((match _ with
+             | @mk_registered _ enc _ _ => enc
+             end s)) with (enc s).
+    all:cbn;try nia.
+  Qed.
+
+End sigTape.
+Hint Resolve sigTape_enc_correct : Lrewrite.
+
+
+From Undecidability Require Import Datatypes.Lists.
+
+Section LMGenNP_to_TMGenNP_mTM.
+  Import EncodeTapes DecodeTapes Single.StepTM ProgrammingTools Combinators Decode.
+  Import LTactics LSum LProd LVector LNat Lists.
+
+  Context (sig:finType) (n:nat) `{R__sig : registered sig}  (M : mTM sig (S n)).
+
+  
+  Definition putFirstAtEnd n: Vector.t (Fin.t (S n)) (S n):=
+    tabulate (fun i => match lt_dec (S (proj1_sig (Fin.to_nat i))) (S n) with
+                      Specif.left H => Fin.of_nat_lt H
+                    | _ => Fin.F1
+                    end).
+  Arguments putFirstAtEnd : simpl never.
+
+  Definition putEndAtFirst n': Vector.t (Fin.t (S n')) (S n'). 
+    refine (tabulate (fun i => match Fin.to_nat i with
+                    | exist _ 0 H => Fin.of_nat_lt (Nat.lt_succ_diag_r n')
+                    | exist _ n' H => Fin.of_nat_lt (p:=n'-1) _
+                            end )). abstract nia.
+  Defined.
+  Arguments putEndAtFirst : simpl never.
+
+  Section printFin.
+    Local Arguments Fin.t : clear implicits.
+    Local Arguments Fin.FS : clear implicits.
+    Local Arguments Fin.F1 : clear implicits.
+    Local Arguments Vector.cast : clear implicits.
+
+    Lemma putFirstAtEnd_dupfree m: dupfree (putFirstAtEnd m).
+    Proof.
+      clear_all. apply dupfree_tabulate_injective.
+      intros i j. destruct (Fin.to_nat i) as [i' Hi] eqn:eqi. destruct (Fin.to_nat j) as [j' Hj] eqn:eqj .
+      cbn. 1:do 2 destruct lt_dec. 2,3:easy.
+      2:{ intros _. apply Fin.to_nat_inj. rewrite eqi. rewrite eqj. cbn. clear eqi eqj. nia. }
+      intros H%Fin.FS_inj. apply Fin.to_nat_inj.
+      rewrite eqi,eqj. cbn. specialize (lt_S_n _ _ l) as H1. specialize (lt_S_n _ _ l0) as H2.
+      erewrite <- (Fin.of_nat_ext H1), <- (Fin.of_nat_ext H2) in H.
+      apply(f_equal Fin.to_nat) in H. rewrite !Fin.to_nat_of_nat in H.
+      now inv H.
+    Qed.
+    
+    Lemma putEndAtFirst_dupfree m: dupfree (putEndAtFirst m).
+    Proof.
+      clear_all. apply dupfree_tabulate_injective.
+      intros i j.
+      destruct (Fin.to_nat i) eqn:?;destruct (Fin.to_nat j) eqn:?; cbn in *.
+      eassert (H'1:=Heqs). assert (H'2:=Heqs0).
+      erewrite <- (Fin.of_nat_to_nat_inv i) in Heqs. erewrite <- (Fin.of_nat_to_nat_inv j) in Heqs0. 
+      rewrite Fin.to_nat_of_nat in Heqs. rewrite Fin.to_nat_of_nat in Heqs0. inversion Heqs; inversion Heqs0.
+            destruct (fin_destruct_S i) as [ (i'&->) | ->]; destruct (fin_destruct_S j) as [ (j'&->) | ->].
+            all:try change (Fin.FS m i') with (Fin.R 1 i') in *; try change (Fin.FS m j') with (Fin.R 1 j') in *.
+            all:change (S m) with (1+m) in *.
+            all: rewrite ?Fin.R_sanity in H0;rewrite ?Fin.R_sanity in H1. all: subst;cbn.
+            all:intros Heq%(f_equal Fin.to_nat).
+            all:rewrite !Fin.to_nat_of_nat in Heq. 
+            all:inversion Heq as [H2]. all:try rewrite ?Nat.sub_0_r in H2.
+            all:try apply Fin.to_nat_inj in H2. all:try easy.
+      -clear - l H2.  nia.
+      -clear - l0 H2.  nia.
+    Qed.
+    
+  End printFin.
+  
+  Definition M__mono : pTM ((sigList (sigTape sig)) ^+) unit 1 :=
+    If (Move R ;; Relabel (MultiToMono.M (LiftTapes (M;(fun _ => tt)) (putEndAtFirst n) )) (Option.apply (fun _ => true) false))
+       Nop
+       Diverge.
+
+  Local Arguments Canonical_Rel : simpl never. 
+  Lemma Realises__mono:
+    M__mono ⊨(fun tin '(_,tout) =>
+              exists v v' : tapes sig (S n),
+                contains_tapes (tape_move_right tin[@Fin0]) v /\
+                contains_tapes tout[@Fin0] v' /\
+                Canonical_Rel (LiftTapes (existT (fun x : mTM sig (S n) => states x -> unit) M (fun _ : states M => tt)) (putEndAtFirst n)) v
+                              (tt, v')).
+  Proof.
+    eapply Realise_monotone.
+    { unfold M__mono. TM_Correct. apply MultiToMono.Realises. } cbn.
+    intros tin ([],tout). cbn. intros [H|H].
+    2:now decompose record H.
+    destruct H as (?&([]&t1&Ht1&b&Hb&H__mono)&<-). destruct b as [ [] | ] ;inv Hb.
+    hnf in H__mono. cbn - [Canonical_Rel]in *|-*. rewrite Ht1 in *|-*. easy.
+  Qed.
+  
+    Lemma Terminates_False sig' n' (M' : mTM sig' n'): M' ↓ (fun _ _ => False).
+  Proof.
+    easy.
+  Qed.
+  
+
+  Lemma Terminates__mono:
+    projT1 M__mono ↓ (fun t k => exists (v : tapes _ (S n)) k',
+                        contains_tapes (tape_move_right t[@Fin0]) v
+                        /\ MultiToMono.Ter (LiftTapes (existT _ M (fun _  => tt)) (putEndAtFirst n))
+                                          (LiftTapes_T (putEndAtFirst n) (Canonical_T M))
+                                          [|(tape_move_right t[@Fin0])|] k'
+                        /\ k' + 3 <= k).
+  Proof.
+    eapply TerminatesIn_monotone.
+    { unfold M__mono. TM_Correct.
+      -apply MultiToMono.Realises.
+      -eapply MultiToMono.Terminates. apply LiftTapes_Terminates. apply putEndAtFirst_dupfree. eapply Canonical_TerminatesIn.
+      -apply Terminates_False.
+    }
+    intros tin k (v&k'&Hv&HT&Hk). cbn.
+    infTer 7. intros t1 _ Ht1. unfold tapes in *. destruct_vector;cbn in *. subst h. apply HT. shelve.
+    intros tout b (?&t1&Ht1&[[]| ]&->&Hr). all:cbn. 2:{ apply Hr. cbn in *. rewrite <- Ht1 in *. easy. } reflexivity.
+    Unshelve.
+    { rewrite <- Hk. nia. } (*
+    hnf in Hr. destruct Hr as (v0&v'&Hv0&Hv'&Hr). replace v0 with v in * by admit.
+    hnf in Hr. cbnunfold LiftTapes in Hr.  cbn in Hr.
+    (*TODO: move trivial relation in Realisation so we get that M terminated if M__Mono halted. *)
+    destruct r
+    2:now decompose record H.
+    destruct H as (?&(b&Hf&H)&<-).
+    destruct b as [[]| ];inv Hf. 
+    destruct H as (v&v'&Hv&Hv'&HR&_).
+    do 3 eexists. 2:split. all:eassumption. *)
+  Qed.
+  
+  
+
+  (*MOVE*)
+  Lemma sizeOfTape_encodeTape sig' (t : tape sig') :
+  | encode_tape t | = let l := sizeOfTape t in if 0 =? l then 1 else 2 + sizeOfTape t.
+  Proof.
+    destruct t;cbn - [Nat.eqb].
+    all:repeat (autorewrite with list;cbn [length]).
+    1:easy.
+    2,3:rewrite !Nat.add_succ_r. all:cbn [Nat.eqb]. all:nia.
+  Qed.
+
+  
+  Lemma sizeOfTape_encodeTape_le sig' (t : tape sig') :
+  | encode_tape t | <= 2 + sizeOfTape t.
+  Proof.
+    rewrite sizeOfTape_encodeTape. cbn;destruct _;nia.
+  Qed.
+
+  Import EqBool.
+
+  Lemma encode_list_concat sigX X (cX : codable sigX X) l:
+    encode_list cX l = concat (map (fun t => sigList_cons :: map sigList_X (encode t)) l) ++[sigList_nil].
+  Proof.
+    induction l;cbn. reflexivity.
+    rewrite IHl. cbn. now autorewrite with list.
+  Qed.
+
+  Lemma list_eq_nth_error X (xs ys : list X) :
+    (forall n, nth_error xs n = nth_error ys n) -> xs = ys.
+  Proof.
+    induction xs in ys|-*;destruct ys;cbn;intros H. 1:easy. 1-2:now specialize (H 0).
+    generalize (H 0).  intros [= ->]. erewrite IHxs. easy. intros n'. now specialize (H (S n')).
+  Qed.
+
+  Lemma vector_nth_error X n' i (xs : Vector.t X n') :
+    nth_error (Vector.to_list xs) i = match lt_dec i n' with
+                                        Specif.left H => Some (Vector.nth xs (Fin.of_nat_lt H))
+                                      | _ => None
+                                      end.
+  Proof.
+    clear. rewrite <- vector_to_list_correct. induction xs in i|-*. now destruct i.
+    cbn in *. destruct i;cbn. easy. rewrite IHxs. do 2 destruct lt_dec. 4:easy. now symmetry;erewrite Fin.of_nat_ext. all:exfalso;nia. 
+  Qed.
+
+  
+  Lemma nth_error_vector X n' i (xs : Vector.t X n') :
+    nth_error (Vector.to_list xs) (proj1_sig (Fin.to_nat i)) = Some (Vector.nth xs i).
+  Proof.
+    clear. rewrite <- vector_to_list_correct. induction xs in i|-*. now inv  i. cbn;rewrite vector_to_list_correct in *.
+    cbn in *. edestruct (fin_destruct_S) as [ (i'&->)| -> ]. 2:now cbn.
+    unshelve erewrite (_ : Fin.FS = Fin.R 1). reflexivity.
+    setoid_rewrite (Fin.R_sanity 1 i'). cbn. easy.
+  Qed.
+    
+
+  Lemma putFirstAtEnd_to_list X n' (x:X) xs:
+    (Vector.to_list (select (putFirstAtEnd n') (x ::: xs))) = Vector.to_list xs ++ [x].
+  Proof.
+    clear. apply list_eq_nth_error. intros i.
+    rewrite !vector_nth_error. destruct lt_dec.
+    { rewrite select_nth. unfold putFirstAtEnd. rewrite nth_tabulate,Fin.to_nat_of_nat;cbn.
+      destruct lt_dec.
+      -erewrite nth_error_app1. 2:now erewrite to_list_length.
+       cbn. rewrite vector_nth_error. destruct lt_dec. 2:exfalso;nia.
+       erewrite Fin.of_nat_ext. reflexivity.
+      -cbn. rewrite nth_error_app2. all:rewrite to_list_length. 2:nia. replace (i-n') with 0 by nia. easy.
+    }
+    symmetry. apply nth_error_None. erewrite app_length, to_list_length. cbn;nia.
+  Qed.
+
+  Lemma putEnd_invL X n' (v : Vector.t X _) :
+    select (putEndAtFirst n') (select (putFirstAtEnd n') v) = v.
+  Proof.
+    apply Vector.eq_nth_iff. intros i ? <-. rewrite !select_nth.
+    f_equal. 
+    unfold putEndAtFirst,putFirstAtEnd. rewrite !nth_tabulate.
+    destruct (fin_destruct_S i) as  [(i'&->) | ->].
+    2:{ cbn. rewrite Fin.to_nat_of_nat. cbn. destruct lt_dec. now exfalso;nia. easy. }
+    eapply Fin.to_nat_inj.
+    remember (Fin.to_nat (Fin.FS i')) as i0 eqn:H. set (tmp:=proj1_sig i0).
+    rewrite (sig_eta i0). subst tmp i0. cbn.
+    destruct (Fin.to_nat i') eqn:H.
+    cbn. rewrite Fin.to_nat_of_nat;cbn. destruct lt_dec;cbn.
+    -rewrite (sig_eta (Fin.to_nat _)). cbn. rewrite Fin.to_nat_of_nat. cbn. nia.
+    -clear H. nia.
+  Qed.
+
+  
+  Lemma right_sizeOfTape sig' (t:tape sig') :
+    length (right t) <= sizeOfTape t.
+  Proof.
+    destruct t;cbn. all:autorewrite with list;cbn. all:nia.
+  Qed.
+  
+
+
+  From Undecidability Require Import MultiUnivTimeSpaceSimulation.
+  Lemma size_list X sigX (cX: codable sigX X) (l:list X) :
+    size l = sumn (map size l) + length l + 1.
+  Proof.
+    unfold size. cbn. rewrite encode_list_concat.
+    rewrite app_length, length_concat, map_map. cbn.
+    change S with (fun x => 1 + x). rewrite sumn_map_add,sumn_map_c. setoid_rewrite map_length.
+    cbn.  nia.
+  Qed.
+
+  Lemma concat_eq_inv_borderL X isBorder xs R__L ys b (R__R : list X):
+    (forall x, x el xs -> exists hd tl, x = hd::tl /\ isBorder hd /\ forall c, c el tl -> ~isBorder c) ->
+    (forall x, x el ys -> exists hd tl, x = hd::tl /\ isBorder hd /\ forall c, c el tl -> ~isBorder c) ->
+    (forall x, x el R__R -> ~isBorder x) ->
+    isBorder b ->
+    concat xs ++ b::R__L = concat ys++R__R ->
+    (forall i, i < length xs -> nth_error xs i = nth_error ys i) /\ b::R__L = concat (skipn (length xs) ys) ++ R__R.
+  Proof.
+    clear. induction xs as [ | x xs] in ys|-*;intros HL HR HRR Hb Heq.
+    { cbn in *. easy. }
+    destruct ys as [ |y ys].
+    { exfalso. cbn in Heq. subst R__R.
+      destruct (HL x) as (?&?&->&?&?). easy. eapply HRR. 2:easy. cbn;easy. }
+    cbn in Heq. autorewrite with list in Heq.
+    destruct (HL x) as (x__hd&x__tl&->&Hxhd&Hxtl). easy.
+    destruct (HR y) as (y__hd&y__tl&->&_&Hytl). easy.
+    cbn in *. 
+    revert Heq. intros [= <- Heq].
+    replace y__tl with x__tl in *.
+    2:{ induction x__tl as [ | x' xtl] in y__tl,Heq,HL,HR,Hytl,Hxtl|-*.
+        -destruct y__tl. easy. cbn in Heq. destruct xs.
+         +now edestruct (Hytl x);inv Heq.
+         +edestruct (HL l) as (?&?&->&?&?). easy. inv Heq. now edestruct Hytl.
+        -destruct y__tl.
+         2:{ inv Heq. f_equal. eapply IHxtl. 3-5:cbn;intros;auto.
+             all:intros z [<-| ].  all:now eauto 7. 
+         }
+         exfalso. destruct ys. 2:{ edestruct (HR l) as (?&?&->&?&?). easy. inv Heq. cbn in *. now eapply Hxtl. }
+         cbn in Heq. 
+         inv Heq. eapply HRR. 2:exact Hb. eauto 10.
+    }
+    apply app_inv_head in Heq. apply IHxs in Heq.  2-5:now eauto 7.
+    destruct Heq as (IH&->). split. 2:easy.
+    intros [] ?. easy. cbn. apply IH. nia.
+  Qed.
+
+  Lemma vector_app_to_list X k k' (xs : Vector.t X k) (ys : Vector.t X k'):
+    vector_to_list (Vector.append xs ys) = vector_to_list xs ++ vector_to_list ys.
+  Proof.   
+    induction xs. easy. cbn. congruence.
+  Qed.
+
+  Lemma putEndAtFirst_to_list X n' v (ts:X) v0:
+    Vector.to_list v ++ [ts] = Vector.to_list v0 ->
+    select (putEndAtFirst n') v0 = ts ::: v.
+  Proof using.
+    intros H. rewrite <- putFirstAtEnd_to_list in H. apply Vectors.vector_to_list_inj in H.
+    subst v0. now setoid_rewrite putEnd_invL.
+  Qed.
+    
+  From Undecidability Require Import UpToC LTactics.
+
+  Section concat.
+    Context X `{registered X}.
+
+    Fixpoint rev_concat acc (xs : list (list X)) :=
+      match xs with
+        [] => acc
+      | x::xs => rev_concat (rev_append x acc) xs
+      end.
+
+    Lemma rev_concat_rev xs acc:
+      rev (rev_concat acc xs) = rev acc ++ concat xs.
+    Proof.
+      induction xs in acc|-*. all:cbn. 2:rewrite IHxs,rev_append_rev. all:autorewrite with list in *. all:easy.
+    Qed.
+
+    Lemma rev_concat_length xs acc:
+      length (rev_concat acc xs) = length acc + length (concat xs).
+    Proof.
+      specialize (rev_concat_rev xs acc) as H1%(f_equal (@length _)).
+      autorewrite with list in H1. nia.
+    Qed.
+
+    
+    Lemma _term_rev_concat :
+      { time : UpToC (fun l => sumn (map (@length _) l) + length l + 1) &
+               computableTime' (@rev_concat) (fun _ _ => (5,fun l _ => (time l,tt)))}.
+    Proof.      
+      evar (c1 : nat).
+      exists_UpToC (fun l => c1 * (sumn (map (@length _) l) + length l + 1) ).
+      { extract. recRel_prettify2.
+        all:cbn - [plus mult].
+        all:enough (c1>=20) by nia.
+        instantiate (c1:=20). all:subst c1;nia. 
+      }
+      smpl_upToC_solve.
+    Qed.
+    Global Instance term_rev_concat : computableTime' rev_concat _ := projT2 _term_rev_concat.
+
+        
+    Lemma _term_concat :
+      { time : UpToC (fun l => sumn (map (@length _) l) + length l + 1) &
+               computableTime' (@concat X) (fun l _ => (time l,tt))}.
+    Proof.
+      eexists_UpToC time. [time]: intros x.
+      eapply computableTimeExt with (x := fun l => rev (rev_concat [] l)).
+      -intros l;hnf. rewrite rev_concat_rev. easy.
+      -extract. solverec. unfold time. reflexivity.
+      -unfold time. setoid_rewrite rev_concat_length. setoid_rewrite length_concat. smpl_upToC_solve.
+    Qed.
+
+    Global Instance term_concat : computableTime' (@concat X) _ := projT2 _term_concat.
+  End concat.
+
+  Section encTape.
+    Context X `{registered X}.  
+    Definition _term_encode_tape : 
+    { time : UpToC (fun l => sizeOfTape l + 1)
+    &   computableTime' (@encode_tape X) (fun l _ => (time l,tt))}.
+    Proof.
+      evar (c1:nat).
+      exists_UpToC (fun l => c1 * sizeOfTape l + c1).
+      {  extract. recRel_prettify. solverec.
+         all:try rewrite !map_time_const. all:autorewrite with list. all:cbn [length].
+         all: ring_simplify. [c1]:exact 42. all:subst c1;nia. }
+      smpl_upToC_solve.
+    Qed.
+
+    Global Instance term_encode_tape : computableTime' (@encode_tape X) _ := projT2 _term_encode_tape.
+
+  End encTape.
+
+  Lemma contains_tapes_inj (sig' : finType) n' t (v v' : tapes sig' n'):
+    contains_tapes t v -> contains_tapes t v' -> v = v'.
+  Proof.
+    unfold contains_tapes. intros -> [= eq]. apply app_inv_tail in eq. apply map_injective in eq. 2:congruence.
+    eassert (H':=encode_prefixInjective (t:=[]) (t':=[])). rewrite !app_nil_r in H'. apply H' in eq. easy.
+  Qed.
+End LMGenNP_to_TMGenNP_mTM.
+
+Arguments putFirstAtEnd : simpl never.
+Arguments putEndAtFirst : simpl never.
