theories/L/TM/TMEncoding.v
@@ -184,6 +184,8 @@ End fix_sig.
 
 Hint Resolve tape_enc_correct : Lrewrite.
 
+From Undecidability Require Import PrettyBounds.SizeBounds.
+
 Lemma sizeOfTape_by_size {sig} `{registered sig} (t:(tape sig)) :
   sizeOfTape t <= size (enc t).
 Proof.
@@ -194,4 +196,13 @@ Proof.
   destruct t. all:cbn [tapeToList length tape_enc size].
   all:rewrite ?app_length,?rev_length. all:cbn [length].
   all:ring_simplify. all:try rewrite !size_list_enc_r. all:try nia.
+Qed.
+
+Lemma sizeOfmTapes_by_size {sig} `{registered sig} n (t:tapes sig n) :
+  sizeOfmTapes t <= size (enc t).
+Proof.
+  setoid_rewrite enc_vector_eq. rewrite size_list.
+  erewrite <- sumn_map_le_pointwise with (f1:=fun _ => _). 2:{ intros. setoid_rewrite <- sizeOfTape_by_size. reflexivity. }
+  rewrite sizeOfmTapes_max_list_map. unfold MaxList.max_list_map. rewrite max_list_sumn.
+  etransitivity. 2:now apply Nat.le_add_r. rewrite vector_to_list_correct. apply sumn_map_le_pointwise. intros. nia.
 Qed.
